Begin replacing 'num' function IDs with a type.
Functions are named/located in a code table from closLang onwards.
Funny arithmetic is done on these numbers to make 'room' for new
allocations. This branch will replace these numbers with a compound
type which will make it easier to allocate a new 'era' with a fresh
set of names available.

Initial progress mostly affects closLang passes.

compiler/backend/clos_numberScript.sml
@@ -1,57 +1,56 @@
 (*
   This simple compiler phase walks the program and gives each closure
-  a unique numeric name.
+  a new unique function identifier.
 *)
 open preamble closLangTheory;
 
 val _ = new_theory"clos_number";
 val _ = set_grammar_ancestry ["closLang"]
 
-(* add fresh code locations *)
-
-val renumber_code_locs_def = tDefine "renumber_code_locs" `
-  (renumber_code_locs_list n [] = (n,[])) /\
-  (renumber_code_locs_list n (x::xs) =
-     let (n,x) = renumber_code_locs n x in
-     let (n,xs) = renumber_code_locs_list n xs in
-     (n, x::xs)) /\
-  (renumber_code_locs n (Var t v) = (n,(Var t v))) /\
-  (renumber_code_locs n (If t x1 x2 x3) =
-     let (n,x1) = renumber_code_locs n x1 in
-     let (n,x2) = renumber_code_locs n x2 in
-     let (n,x3) = renumber_code_locs n x3 in
-       (n,If t x1 x2 x3)) /\
-  (renumber_code_locs n (Let t xs x2) =
-     let (n,xs) = renumber_code_locs_list n xs in
-     let (n,x2) = renumber_code_locs n x2 in
-       (n,Let t xs x2)) /\
-  (renumber_code_locs n (Raise t x1) =
-     let (n,x1) = renumber_code_locs n x1 in
-       (n,Raise t x1)) /\
-  (renumber_code_locs n (Tick t x1) =
-     let (n,x1) = renumber_code_locs n x1 in
-       (n,Tick t x1)) /\
-  (renumber_code_locs n (Op t op xs) =
-     let (n,xs) = renumber_code_locs_list n xs in
-       (n,Op t op xs)) /\
-  (renumber_code_locs n (App t loc_opt x1 x2) =
-     let (n,x1) = renumber_code_locs n x1 in
-     let (n,x2) = renumber_code_locs_list n x2 in
-       (n,App t NONE x1 x2)) /\
-  (renumber_code_locs n (Fn t loc vs num_args x1) =
-     let (n,x1) = renumber_code_locs n x1 in
-       (n+2,Fn t (SOME n) vs num_args x1)) /\
-  (renumber_code_locs n (Letrec t loc vs fns x1) =
-     let (m,fns') = renumber_code_locs_list n (MAP SND fns) in
-     let (n,x1) = renumber_code_locs (m+2*LENGTH fns') x1 in
-       (n,Letrec t (SOME m) vs (ZIP (MAP FST fns, fns')) x1)) /\
-  (renumber_code_locs n (Handle t x1 x2) =
-     let (n,x1) = renumber_code_locs n x1 in
-     let (n,x2) = renumber_code_locs n x2 in
-       (n,Handle t x1 x2)) /\
-  (renumber_code_locs n (Call t ticks dest xs) =
-     let (n,xs) = renumber_code_locs_list n xs in
-       (n,Op t Add xs)) (* this case cannot occur *)`
+val renumber_code_fnames_def = tDefine "renumber_code_fnames" `
+  (renumber_code_fnames_list nm [] = (nm,[])) /\
+  (renumber_code_fnames_list nm (x::xs) =
+     let (nm,x) = renumber_code_fnames nm x in
+     let (nm,xs) = renumber_code_fnames_list nm xs in
+     (nm, x::xs)) /\
+  (renumber_code_fnames nm (Var t v) = (nm,(Var t v))) /\
+  (renumber_code_fnames nm (If t x1 x2 x3) =
+     let (nm,x1) = renumber_code_fnames nm x1 in
+     let (nm,x2) = renumber_code_fnames nm x2 in
+     let (nm,x3) = renumber_code_fnames nm x3 in
+       (nm,If t x1 x2 x3)) /\
+  (renumber_code_fnames nm (Let t xs x2) =
+     let (nm,xs) = renumber_code_fnames_list nm xs in
+     let (nm,x2) = renumber_code_fnames nm x2 in
+       (nm,Let t xs x2)) /\
+  (renumber_code_fnames nm (Raise t x1) =
+     let (nm,x1) = renumber_code_fnames nm x1 in
+       (nm,Raise t x1)) /\
+  (renumber_code_fnames nm (Tick t x1) =
+     let (nm,x1) = renumber_code_fnames nm x1 in
+       (nm,Tick t x1)) /\
+  (renumber_code_fnames nm (Op t op xs) =
+     let (nm,xs) = renumber_code_fnames_list nm xs in
+       (nm,Op t op xs)) /\
+  (renumber_code_fnames nm (App t fn_opt x1 x2) =
+     let (nm,x1) = renumber_code_fnames nm x1 in
+     let (nm,x2) = renumber_code_fnames_list nm x2 in
+       (nm,App t NONE x1 x2)) /\
+  (renumber_code_fnames nm (Fn t fn_opt vs num_args x1) =
+     let (nm,x1) = renumber_code_fnames nm x1 in
+       (next_fname nm 2,Fn t (SOME nm) vs num_args x1)) /\
+  (renumber_code_fnames nm (Letrec t fn_opt vs fns x1) =
+     let (start_nm,fns') = renumber_code_fnames_list nm (MAP SND fns) in
+     let next_nm = next_fname start_nm (2 * LENGTH fns') in
+     let (nm,x1) = renumber_code_fnames next_nm x1 in
+       (nm,Letrec t (SOME start_nm) vs (ZIP (MAP FST fns, fns')) x1)) /\
+  (renumber_code_fnames nm (Handle t x1 x2) =
+     let (nm,x1) = renumber_code_fnames nm x1 in
+     let (nm,x2) = renumber_code_fnames nm x2 in
+       (nm,Handle t x1 x2)) /\
+  (renumber_code_fnames nm (Call t ticks dest xs) =
+     let (nm,xs) = renumber_code_fnames_list nm xs in
+       (nm,Op t Add xs)) (* this case cannot occur *)`
  (WF_REL_TAC `inv_image $< (λx. case x of INL p => exp3_size (SND p) | INR p => exp_size (SND p))` >>
  rw [] >>
  TRY decide_tac >>
@@ -61,13 +60,16 @@ val renumber_code_locs_def = tDefine "renumber_code_locs" `
  rw [exp_size_def] >>
  decide_tac);
 
-val renumber_code_locs_ind = theorem"renumber_code_locs_ind";
+val renumber_code_fnames_ind = theorem"renumber_code_fnames_ind";
 
-Theorem renumber_code_locs_length
-  `(∀x y. LENGTH (SND (renumber_code_locs_list x y)) = LENGTH y) ∧
-    (∀(x:num)(y:closLang$exp). T)`
-    (ho_match_mp_tac renumber_code_locs_ind >>
-    simp[renumber_code_locs_def,UNCURRY] >> rw[] >>
+val renumber_code_fnames_ind1 = renumber_code_fnames_ind
+  |> Q.SPECL [`P`, `\_ _. T`] 
+  |> UNDISCH_ALL |> CONJUNCT1 |> DISCH_ALL;
+
+Theorem renumber_code_fnames_length
+  `(∀x y. LENGTH (SND (renumber_code_fnames_list x y)) = LENGTH y)`
+    (ho_match_mp_tac renumber_code_fnames_ind1 >>
+    simp[renumber_code_fnames_def,UNCURRY] >> rw[] >>
     METIS_TAC[PAIR,FST,SND]);
 
 val _ = export_theory()
