compiler/backend/clos_labelsScript.sml
@@ -4,10 +4,10 @@
 open preamble closLangTheory;
 
 val _ = new_theory "clos_labels";
-val _ = set_grammar_ancestry ["closLang","misc","sptree"];
+val _ = set_grammar_ancestry ["closLang","misc","backend_common"];
 
 val remove_dests_def = tDefine "remove_dests" `
-  (remove_dests (ds:num_set) [] = []) /\
+  (remove_dests (ds: unit fntree) [] = []) /\
   (remove_dests ds ((x:closLang$exp)::y::xs) =
      HD (remove_dests ds [x]) :: remove_dests ds (y::xs)) /\
   (remove_dests ds [Var t v] = [Var t v]) /\
@@ -28,71 +28,72 @@ val remove_dests_def = tDefine "remove_dests" `
      [Op t op (remove_dests ds xs)]) /\
   (remove_dests ds [Tick t x] = [Tick t (HD (remove_dests ds [x]))]) /\
   (remove_dests ds [Call t ticks dest xs] =
-   if IS_SOME (lookup dest ds) then
+   if IS_SOME (fntree_lookup dest ds) then
     [Call t ticks dest (remove_dests ds xs)]
    else [Op t (if NULL xs then El else String "") (remove_dests ds xs)]) /\
   (remove_dests ds [App t NONE x1 xs] =
   [App t NONE (HD (remove_dests ds [x1])) (remove_dests ds xs)]) /\
   (remove_dests ds [App t (SOME dest) x1 xs] =
-  if IS_SOME (lookup dest ds) then
+  if IS_SOME (fntree_lookup dest ds) then
     [App t (SOME dest) (HD (remove_dests ds [x1])) (remove_dests ds xs)]
   else
     if NULL xs then [Let t [Op t El []] (HD (remove_dests ds [x1]))]
     else [Op t (String"") (remove_dests ds xs ++ remove_dests ds [x1])]) /\
-  (remove_dests ds [Letrec t loc_opt vs fns x1] =
+  (remove_dests ds [Letrec t fn_opt vs fns x1] =
      let m = LENGTH fns in
      let new_fns =
        MAP (\(num_args, x).
          (num_args, HD (remove_dests ds [x]))) fns in
-     [Letrec t loc_opt vs new_fns (HD (remove_dests ds [x1]))]) /\
-  (remove_dests ds [Fn t loc_opt vs num_args x1] =
-    [Fn t loc_opt vs num_args (HD (remove_dests ds [x1]))])`
+     [Letrec t fn_opt vs new_fns (HD (remove_dests ds [x1]))]) /\
+  (remove_dests ds [Fn t fn_opt vs num_args x1] =
+    [Fn t fn_opt vs num_args (HD (remove_dests ds [x1]))])`
   (WF_REL_TAC `measure (exp3_size o SND)`
    \\ simp []
    \\ rpt strip_tac
    \\ imp_res_tac exp1_size_lemma
    \\ simp []);
 
-val add_code_locs_def = tDefine "add_code_locs" `
-  (add_code_locs ds [] = ds) /\
-  (add_code_locs ds (x::y::xs) =
-     let ds = add_code_locs ds [x] in
-       add_code_locs ds (y::xs)) /\
-  (add_code_locs ds [Var _ v] = ds) /\
-  (add_code_locs ds [If _ x1 x2 x3] =
-     let ds = add_code_locs ds [x1] in
-     let ds = add_code_locs ds [x2] in
-     let ds = add_code_locs ds [x3] in
+val add_code_names_def = tDefine "add_code_names" `
+  (add_code_names ds [] = ds) /\
+  (add_code_names ds (x::y::xs) =
+     let ds = add_code_names ds [x] in
+       add_code_names ds (y::xs)) /\
+  (add_code_names ds [Var _ v] = ds) /\
+  (add_code_names ds [If _ x1 x2 x3] =
+     let ds = add_code_names ds [x1] in
+     let ds = add_code_names ds [x2] in
+     let ds = add_code_names ds [x3] in
        ds) /\
-  (add_code_locs ds [Let _ xs x2] =
-     let ds = add_code_locs ds xs in
-     let ds = add_code_locs ds [x2] in
+  (add_code_names ds [Let _ xs x2] =
+     let ds = add_code_names ds xs in
+     let ds = add_code_names ds [x2] in
        ds) /\
-  (add_code_locs ds [Raise _ x1] =
-     add_code_locs ds [x1]) /\
-  (add_code_locs ds [Tick _ x1] =
-     add_code_locs ds [x1]) /\
-  (add_code_locs ds [Op _ op xs] =
-     add_code_locs ds xs) /\
-  (add_code_locs ds [App _ loc_opt x1 xs] =
-     let ds = add_code_locs ds [x1] in
-     let ds = add_code_locs ds xs in
+  (add_code_names ds [Raise _ x1] =
+     add_code_names ds [x1]) /\
+  (add_code_names ds [Tick _ x1] =
+     add_code_names ds [x1]) /\
+  (add_code_names ds [Op _ op xs] =
+     add_code_names ds xs) /\
+  (add_code_names ds [App _ fn_opt x1 xs] =
+     let ds = add_code_names ds [x1] in
+     let ds = add_code_names ds xs in
        ds) /\
-  (add_code_locs ds [Fn _ loc_opt vs num_args x1] =
-     let loc = case loc_opt of NONE => 0 | SOME n => n in
-     let ds = add_code_locs ds [x1] in
-       insert loc () ds) /\
-  (add_code_locs ds [Letrec _ loc_opt vs fns x1] =
-     let loc = case loc_opt of NONE => 0 | SOME n => n in
-     let ds = add_code_locs ds (MAP SND fns) in
-     let ds = add_code_locs ds [x1] in
-       list_insert (GENLIST (λn. loc + 2*n) (LENGTH fns)) ds) /\
-  (add_code_locs ds [Handle _ x1 x2] =
-     let ds = add_code_locs ds [x1] in
-     let ds = add_code_locs ds [x2] in
+  (add_code_names ds [Fn _ fn_opt vs num_args x1] =
+     let ds = add_code_names ds [x1] in
+     case fn_opt of NONE => ds
+       | SOME fname => fntree_insert fname () ds) /\
+  (add_code_names ds [Letrec _ fn_opt vs fns x1] =
+     let ds = add_code_names ds (MAP SND fns) in
+     let ds = add_code_names ds [x1] in
+     case fn_opt of NONE => ds
+       | SOME fname => fntree_list_insert
+         (GENLIST (\n. next_fname fname (2 * n)) (LENGTH fns)) ds) /\
+  (add_code_names ds [Handle _ x1 x2] =
+     let ds = add_code_names ds [x1] in
+     let ds = add_code_names ds [x2] in
        ds) /\
-  (add_code_locs ds [Call _ ticks dest xs] =
-     add_code_locs ds xs)`
+  (add_code_names ds [Call _ ticks dest xs] =
+     add_code_names ds xs)`
   (WF_REL_TAC `measure (exp3_size o SND)`
    \\ REPEAT STRIP_TAC \\ TRY DECIDE_TAC >>
    Induct_on `fns` >>
@@ -103,8 +104,8 @@ val add_code_locs_def = tDefine "add_code_locs" `
 
 val compile_def = Define`
   compile prog =
-    let ds = list_insert (MAP FST prog) LN in
-    let ds = add_code_locs ds (MAP (SND o SND) prog) in
+    let ds = fntree_list_insert (MAP FST prog) LN in
+    let ds = add_code_names ds (MAP (SND o SND) prog) in
       MAP (λ(n,args,exp). (n, args, HD(remove_dests ds [exp]))) prog`;
 
 Theorem LENGTH_remove_dests
